progress with concrete encoding
implement `decode_pair` (subject to change, may not have further desired properties)
remove unused (demo) lemma

papers/116_stefan_rass/LD_Issues.thy
@@ -3,24 +3,52 @@ theory LD_Issues
 begin
 
 
-\<comment> \<open>Decode a pair of words \<open>(l, x) \<in> {0,1}* \<times> {0,1}*\<close> from its encoded form "\<open>l\<parallel>x \<in> {0,1}*\<close>".
+\<comment> \<open>Decode a pair of \<open>(l, x) \<in> \<nat> \<times> {0,1}*\<close> from its encoded form \<open>w \<in> {0,1}*\<close>.
 
   The encoding defined by this should have \<open>l\<close> encoded in the upper (more significant) bits of \<open>l\<parallel>x\<close>.
 
-  This is undefined for now, as the restricted alphabet does not allow the obvious method
-  of using a separation symbol that can not occur in \<open>l\<close>.
-  (It suffices to restrict this condition to \<open>l\<close>, since after encountering the symbol
-  the "rest" of \<open>w\<close> is determined \<open>x\<close>.)
+  \<open>w\<close> is related to \<open>(l, x)\<close> through the regular expression \<open>1\<^sup>l0x{0,1}\<^sup>k\<close>,
+  where \<^term>\<open>k = suffix_len w\<close>.
+  If \<open>w\<close> does not match the expression, default values \<open>l = 0, x = []\<close> are assigned.
 
-  A possible solution for this would be to use another encoding for \<open>l\<close>,
-  such as \<^const>\<open>decode_word\<close>, defined in \<^theory>\<open>OWF.Complexity\<close>.
-  However, this method may have unintended side-effects, as the encoding increases the length,
-  which is critical in proving some of the further lemmas.\<close>
+  Construction:
+  To ensure the required property for Lemma 4.6, the lower ~half of \<open>w\<close>
+  (the \<^term>\<open>suffix_len w\<close> least-significant-bits) is dropped.
+  Then, \<open>l\<close> is the number of leading \<open>1\<close>s.
+  Remove all leading \<open>1\<close>s and one \<open>0\<close> to retain \<open>x\<close>.\<close>
 
-\<comment> \<open>what if \<open>l = 1\<^sup>n\<close> and \<open>\<cent> = 0\<close>? then \<open>w = 1\<^sup>l0w\<close>\<close>
+definition strip_sq_pad :: "word \<Rightarrow> word"
+  where "strip_sq_pad w \<equiv> drop (suffix_len w) w"
 
-definition decode_pair :: "word \<Rightarrow> word \<times> word"
-  where "decode_pair \<equiv> undefined"
+definition decode_pair_l :: "word \<Rightarrow> nat"
+  where "decode_pair_l w = length (takeWhile (\<lambda>x. x = True) (rev (strip_sq_pad w)))"
+
+definition decode_pair_x :: "word \<Rightarrow> word"
+  where "decode_pair_x w = rev (tl (dropWhile (\<lambda>x. x = True) (rev (strip_sq_pad w))))"
+
+abbreviation decode_pair :: "word \<Rightarrow> nat \<times> word"
+  where "decode_pair w \<equiv> (decode_pair_l w, decode_pair_x w)"
+
+
+lemma pair_adj_sq_eq:
+  fixes w
+  defines w': "w' \<equiv> adj_sq\<^sub>w w"
+  assumes len: "length w \<ge> 9"
+  shows "decode_pair w' = decode_pair w"
+proof -
+  let ?sl = "suffix_len w" and ?lw = "length w" and ?lw' = "length w'"
+  from len have sh: "shared_MSBs (?lw - ?sl) w w'" unfolding w' by (rule adj_sq_sh_pfx_half)
+  from sh have l_eq: "?lw' = ?lw" ..
+
+  from len have "?sl \<le> length w" by (rule suffix_min_len)
+  then have "?lw - (?lw - ?sl) = ?sl" by (rule diff_diff_cancel)
+  from sh have "drop (?lw' - (?lw - ?sl)) w' = drop (?lw - (?lw - ?sl)) w" ..
+  then have "drop ?sl w' = drop ?sl w" unfolding l_eq \<open>?lw - (?lw - ?sl) = ?sl\<close> .
+  then have sq_pad_eq: "strip_sq_pad w' = strip_sq_pad w"
+    unfolding strip_sq_pad_def suffix_len_def l_eq .
+  show "decode_pair w' = decode_pair w"
+    unfolding decode_pair_x_def decode_pair_l_def sq_pad_eq ..
+qed
 
 
 context tht_assms
@@ -29,12 +57,12 @@ begin
 \<comment> \<open>Alternative \<open>L\<^sub>D\<close>.
 
   Note: this is not intended to replace \<^const>\<open>L\<^sub>D\<close>.
-  The further proof uses the similarity of \<open>L\<^sub>D\<close> and \<open>L\<^sub>D''\<close>
+  Instead, the further proof uses the similarity of \<open>L\<^sub>D\<close> and \<open>L\<^sub>D''\<close>
   to prove properties of \<open>L\<^sub>D''\<close> via reduction to \<open>L\<^sub>D\<close>.
 
   Construction: Given a word \<open>w\<close>.
-  Split the word \<open>w\<close> into \<open>(l, x)\<close> using \<^const>\<open>decode_pair\<close>.
-  Define \<open>v\<close> as the \<open>log\<^sub>2(l)\<close> most-significant-bits of \<open>x\<close>.
+  Split the word \<open>w\<close> into \<open>(l::nat, x::word)\<close> using \<^const>\<open>decode_pair\<close>.
+  Define \<open>v\<close> as the \<open>l\<close> most-significant-bits of \<open>x\<close>.
   Remove the arbitrary-length \<open>1\<^sup>+0\<close>-prefix from \<open>v\<close> to retain the pure encoding of \<open>M\<^sub>v\<close>.
   If \<open>M\<^sub>v\<close> rejects \<open>v\<close> within \<open>T(len(x))\<close> steps, \<open>w \<in> L\<^sub>D''\<close> holds.
 
@@ -43,74 +71,21 @@ begin
   The alternative version shown in @{thm time_bounded_altdef} is used for simplicity.\<close>
 
 definition (in tht_assms) L\<^sub>D'' :: lang
-  where "L\<^sub>D'' \<equiv> {w. 
+  where "L\<^sub>D'' \<equiv> {w.
       let (l, x) = decode_pair w;
-          v = drop (length x - clog (l)\<^sub>2) x;
+          v = drop (length x - l) x;
           M\<^sub>v = decode_TM (strip_al_prefix v) in
       rejects M\<^sub>v v \<and> is_final (steps0 (1, <v>\<^sub>t\<^sub>p) M\<^sub>v (tcomp\<^sub>w T x))
     }"
 
+lemma L\<^sub>D''_adj_sq_iff:
+  fixes w
+  defines w': "w' \<equiv> adj_sq\<^sub>w w"
+  assumes len: "length w \<ge> 9"
+  shows "w' \<in> L\<^sub>D'' \<longleftrightarrow> w \<in> L\<^sub>D''"
+  unfolding L\<^sub>D''_def mem_Collect_eq w' len[THEN pair_adj_sq_eq] ..
+
 end \<comment> \<open>\<^locale>\<open>tht_assms\<close>\<close>
 
-
-context tht_sq_assms
-begin
-
-lemma
-  fixes w
-  defines "w' \<equiv> adj_sq\<^sub>w w"
-  defines "l \<equiv> fst (decode_pair w)"
-    and "x \<equiv> snd (decode_pair w)"
-    and "l' \<equiv> fst (decode_pair w')"
-    and "x' \<equiv> snd (decode_pair w')"
-  defines "v \<equiv> drop (length x - clog (l)\<^sub>2) x"
-    and "v' \<equiv> drop (length x' - clog (l')\<^sub>2) x'"
-    (* need some assumption that fixes the length of l in a way that allows this to work *)
-  shows "v' = v"
-proof -
-  oops
-
-
-lemma L\<^sub>D_adj_sq_iff:
-  fixes w
-  defines l: "l \<equiv> fst (decode_pair w)"
-    and w': "w' \<equiv> adj_sq\<^sub>w w"
-  assumes "length w \<ge> 20"
-    and "clog (l)\<^sub>2 \<le> clog (length w)" (* new *)
-  shows "w' \<in> L\<^sub>D'' \<longleftrightarrow> w \<in> L\<^sub>D''"
-proof -
-  from \<open>length w \<ge> 20\<close> have "shared_MSBs (clog (length w)) w w'" unfolding w' by (rule adj_sq_sh_pfx_log)
-  then have "length w' = length w" by (elim sh_msbE[symmetric])
-  oops
-
-end \<comment> \<open>\<^locale>\<open>tht_sq_assms\<close>\<close>
-
-
-lemma (* relation between two similar, but not equivalent propositions *)
-  assumes "tm_wf0 M_w"
-    and "M_w \<noteq> Rejecting_TM"
-  shows "TM_decode_pad w = M_w \<longleftrightarrow> strip_al_prefix (strip_exp_pad w) = encode_TM M_w"
-proof (rule iffI)
-  assume *: "TM_decode_pad w = M_w"
-  with assms(2) have h1: "is_encoded_TM (strip_al_prefix (strip_exp_pad w))"
-    unfolding TM_decode_pad_def decode_TM_def by argo
-
-  then have h2: "\<exists>!M. strip_al_prefix (strip_exp_pad w) = encode_TM M"
-    unfolding is_encoded_TM_def apply (rule ex_ex1I)
-    using encode_TM_inj unfolding inj_def by presburger
-
-  from assms(2) * have h3: "tm_wf0 (THE M. strip_al_prefix (strip_exp_pad w) = encode_TM M)"
-    unfolding TM_decode_pad_def decode_TM_def h1[THEN if_P] filter_wf_TMs_def by argo
-
-  show "strip_al_prefix (strip_exp_pad w) = encode_TM M_w"
-    unfolding *[symmetric] TM_decode_pad_def
-    unfolding decode_TM_def h1[THEN if_P]
-    unfolding filter_wf_TMs_def h3[THEN if_P]
-    using h2[THEN theI_unique] by blast
-next
-  assume *: "strip_al_prefix (strip_exp_pad w) = encode_TM M_w"
-  show "TM_decode_pad w = M_w" unfolding TM_decode_pad_def *
-    by (rule codec_TM) fact
-qed
 
 end
